Refactor controlbits C for porting.

c/bindings.cpp
@@ -4,24 +4,15 @@
 #include <stdlib.h>
 #include <string.h>
 extern "C" {
-#include "crypto_kem.h"
-#include "operations.h"
-
-#include "controlbits.h"
-#include "randombytes.h"
 #include "crypto_hash.h"
-#include "encrypt.h"
-#include "decrypt.h"
+#include "gf.h"
+#include "int32_sort.h"
 #include "params.h"
-#include "sk_gen.h"
-#include "uint64_sort.h"
 #include "util.h"
-#include "transpose.h"
 
 #include <openssl/conf.h>
 #include <openssl/evp.h>
 #include <openssl/err.h>
-
 }
 #include <gmp.h>
 
@@ -314,6 +305,180 @@ extern "C" lean_obj_res lean_store_gf(b_lean_obj_arg irr_obj) {
     return sk_obj;
 }
 
+/* input: p, an array of int16 */
+/* input: n, length of p */
+/* input: s, meaning that stride-2^s cswaps are performed */
+/* input: cb, the control bits */
+/* output: the result of apply the control bits to p */
+static void layer(int16_t *p, const unsigned char *cb, int s, int n) {
+  const int stride = 1 << s;
+  int index = 0;
+
+  for (int i = 0; i < n; i += stride*2) {
+    for (int j = 0; j < stride; j++) {
+      int16_t d = p[ i+j ] ^ p[ i+j+stride ];
+      int16_t m = (cb[ index >> 3 ] >> (index & 7)) & 1;
+      m = -m;
+      d &= m;
+      p[ i+j ] ^= d;
+      p[ i+j+stride ] ^= d;
+      index++;
+    }
+  }
+}
+
+/* parameters: 1 <= w <= 14; n = 2^w */
+/* input: permutation pi of {0,1,...,n-1} */
+/* output: (2m-1)n/2 control bits at positions pos,pos+step,... */
+/* output position pos is by definition 1&(out[pos/8]>>(pos&7)) */
+/* caller must 0-initialize positions first */
+/* temp must have space for int32[2*n] */
+static void cbrecursion(unsigned char *out,long long pos,long long step,const int16_t *pi,long long w,long long n,int32_t *temp) {
+    // A refers to the first n elements in temp.
+    int32_t* A = temp;
+    // B refers tot he second n elemnts in temp.
+    int32_t* B = temp+n;
+
+
+    if (w == 1) {
+        out[pos>>3] ^= pi[0]<<(pos&7);
+        return;
+    }
+
+    for (long long x = 0;x < n;++x)
+        A[x] = ((pi[x]^1)<<16)|pi[x^1];
+
+
+    int32_sort(A,n); /* A = (id<<16)+pibar */
+
+    for (long long x = 0; x < n; ++x) {
+        int32_t Ax = A[x];
+        int32_t px = Ax&0xffff;
+        int32_t cx = px;
+        if (x < cx) cx = x;
+        B[x] = (px<<16)|cx;
+    }
+    /* B = (p<<16)+c */
+
+    for (long long x = 0; x < n; ++x)
+        A[x] = (A[x]<<16)|x; /* A = (pibar<<16)+id */
+    int32_sort(A,n); /* A = (id<<16)+pibar^-1 */
+
+    for (long long x = 0; x < n; ++x)
+        A[x] = (A[x]<<16)+(B[x]>>16); /* A = (pibar^(-1)<<16)+pibar */
+    int32_sort(A,n); /* A = (id<<16)+pibar^2 */
+
+    if (w <= 10) {
+        for (long long x = 0;x < n;++x)
+            B[x] = ((A[x]&0xffff)<<10)|(B[x]&0x3ff);
+
+        for (long long i = 1;i < w-1;++i) {
+            /* B = (p<<10)+c */
+
+            for (long long x = 0; x < n; ++x)
+                A[x] = ((B[x]&~0x3ff)<<6)|x; /* A = (p<<16)+id */
+            int32_sort(A,n); /* A = (id<<16)+p^{-1} */
+
+            for (long long x = 0;x < n;++x)
+                A[x] = (A[x]<<20)|B[x]; /* A = (p^{-1}<<20)+(p<<10)+c */
+            int32_sort(A,n); /* A = (id<<20)+(pp<<10)+cp */
+
+            for (long long x = 0; x < n; ++x) {
+                int32_t ppcpx = A[x]&0xfffff;
+                int32_t ppcx = (A[x]&0xffc00)|(B[x]&0x3ff);
+                if (ppcpx < ppcx) ppcx = ppcpx;
+                B[x] = ppcx;
+            }
+        }
+        for (long long x = 0;x < n;++x)
+            B[x] &= 0x3ff;
+    } else {
+        for (long long x = 0;x < n;++x)
+            B[x] = (A[x]<<16)|(B[x]&0xffff);
+
+        for (long long i = 1;i < w-1;++i) {
+            /* B = (p<<16)+c */
+
+            for (long long x = 0;x < n;++x)
+                A[x] = (B[x]&~0xffff)|x;
+            int32_sort(A,n); /* A = (id<<16)+p^(-1) */
+
+            for (long long x = 0;x < n;++x)
+                A[x] = (A[x]<<16)|(B[x]&0xffff);
+            /* A = p^(-1)<<16+c */
+
+            if (i < w-2) {
+                for (long long x = 0;x < n;++x)
+                    B[x] = (A[x]&~0xffff)|(B[x]>>16);
+                /* B = (p^(-1)<<16)+p */
+                int32_sort(B,n); /* B = (id<<16)+p^(-2) */
+                for (long long x = 0; x < n; ++x)
+                    B[x] = (B[x]<<16)|(A[x]&0xffff);
+                /* B = (p^(-2)<<16)+c */
+            }
+
+            int32_sort(A,n);
+            /* A = id<<16+cp */
+            for (long long x = 0;x < n;++x) {
+                int32_t cpx = (B[x]&~0xffff)|(A[x]&0xffff);
+                if (cpx < B[x]) B[x] = cpx;
+            }
+        }
+        for (long long x = 0;x < n;++x) B[x] &= 0xffff;
+    }
+
+    for (long long x = 0;x < n;++x) A[x] = (((int32_t)pi[x])<<16)+x;
+    int32_sort(A,n); /* A = (id<<16)+pi^(-1) */
+
+    for (long long j = 0;j < n/2;++j) {
+        long long x = 2*j;
+        int32_t fj = B[x]&1; /* f[j] */
+        int32_t Fx = x+fj; /* F[x] */
+        int32_t Fx1 = Fx^1; /* F[x+1] */
+
+        out[pos>>3] ^= fj<<(pos&7);
+        pos += step;
+
+        B[x] = (A[x]<<16)|Fx;
+        B[x+1] = (A[x+1]<<16)|Fx1;
+    }
+    /* B = (pi^(-1)<<16)+F */
+    int32_sort(B,n); /* B = (id<<16)+F(pi) */
+
+    pos += (2*w-3)*step*(n/2);
+
+    for (long long k = 0;k < n/2;++k) {
+        long long y = 2*k;
+        int32_t lk = B[y]&1; /* l[k] */
+        int32_t Ly = y+lk; /* L[y] */
+        int32_t Ly1 = Ly^1; /* L[y+1] */
+
+        out[pos>>3] ^= lk<<(pos&7);
+        pos += step;
+
+        A[y] = (Ly<<16)|(B[y]&0xffff);
+        A[y+1] = (Ly1<<16)|(B[y+1]&0xffff);
+    }
+    /* A = (L<<16)+F(pi) */
+
+    int32_sort(A,n); /* A = (id<<16)+F(pi(L)) = (id<<16)+M */
+
+    // We will only need n elements in temp in recursive calls (instead of 2*n)
+    // and we no longer need B, so we use it for storing new pi value.
+    // q has n int16_t elements, so it only need n/2 int32_t elements from B.
+    /* q can start anywhere between temp+n and temp+n+n/2 */
+    int16_t* q = (int16_t *) (B);
+
+    pos -= (2*w-2)*step*(n/2);
+    for (long long j = 0;j < n/2;++j) {
+        q[j] = (A[2*j]&0xffff)>>1;
+        q[j+n/2] = (A[2*j+1]&0xffff)>>1;
+    }
+
+    cbrecursion(out,pos,step*2,q,w-1,n/2,temp);
+    cbrecursion(out,pos+step,step*2,q+n/2,w-1,n/2,temp);
+}
+
 extern "C" lean_obj_res lean_controlbitsfrompermutation(b_lean_obj_arg pi_obj) {
 
     const size_t perm_count = 1 << GFBITS;
@@ -323,12 +488,43 @@ extern "C" lean_obj_res lean_controlbitsfrompermutation(b_lean_obj_arg pi_obj) {
         pi[i] = lean_unbox_uint32(lean_array_get_core(pi_obj, i));
     }
 
-    lean_obj_res sk_obj = lean_alloc_sarray1(1, COND_BYTES);
-    uint8_t* sk = lean_sarray_cptr(sk_obj);
+    lean_obj_res out_obj = lean_alloc_sarray1(1, COND_BYTES);
+    uint8_t* out = lean_sarray_cptr(out_obj);
 
-    controlbitsfrompermutation(sk, pi, GFBITS, 1 << GFBITS);
+    long long w = GFBITS;
+    long long n = 1 << GFBITS;
 
-    return sk_obj;
+    int32_t temp[2*n];
+    memset(out,0, COND_BYTES);
+    cbrecursion(out,0,1,pi,w,n,temp);
+
+    // check for correctness
+
+    int16_t pi_test[n];
+    for (int i = 0; i < n; i++)
+    pi_test[i] = i;
+
+    unsigned char *ptr = out;
+    for (int i = 0; i < w; i++) {
+        layer(pi_test, ptr, i, n);
+        ptr += n >> 4;
+    }
+
+    for (int i = w-2; i >= 0; i--) {
+        layer(pi_test, ptr, i, n);
+        ptr += n >> 4;
+    }
+
+    int16_t diff = 0;
+    for (int i = 0; i < n; i++)
+        diff |= pi[i] ^ pi_test[i];
+
+    if (diff != 0) {
+        lean_dec_ref(out_obj);
+        return lean_mk_option_none();
+    }
+
+    return lean_mk_option_some(out_obj);
 }
 
 /* input: in, a 64x64 matrix over GF(2) */
